coq-osiris/theories/stdlib/Stdlib.v
@@ -150,10 +150,10 @@ Definition decide_spec `{Encode A}
 :=
   ∀ (x : A),
     P x →
-    pure (call decide #x) (λ v,
+    pure_enc (call decide #x) (λ v,
       ∀ (y : A),
       P y →
-      pure (call v #y) (λ (b : bool),
+      pure_enc (call v #y) (λ (b : bool),
         b ↔ R x y
       )
     ).
@@ -168,7 +168,7 @@ Local Lemma decide_spec' `{Encode A}
 :
   decide_spec decide P R →
   ∀ (x y : A), P x → P y →
-  pure
+  pure_enc
     (bind (call decide #x) (λ v, call v #y))
     (λ (b : bool),
       b ↔ R x y
@@ -192,8 +192,8 @@ Definition compare_spec `{Encode A} (compare : val) (le : A → A → Prop) :=
   let lt := strict le in
   let eq := equivalent le in
   ∀ (x y : A),
-    pure (call compare #x) (λ v,
-        pure (call v #y) (λ (c : Z),
+    pure_enc (call compare #x) (λ v,
+        pure_enc (call v #y) (λ (c : Z),
             representable c ∧
               (c < 0 ↔ lt x y)%Z ∧
               (c = 0 ↔ eq x y)%Z ∧
@@ -296,7 +296,7 @@ Qed.
    first argument is pure, so its specification is expressed using pure. *)
 
 Lemma Stdlib__store__spec (l : loc) (v v' : val) :
-  pure
+  pure_enc
     (call Stdlib__store #l)
     (λ c,
       {{{ l ↦ V v }}}
